Ugly proof of Append Entries case of allEntries->logs

raft/proof/AllEntriesVotesWithLogProof.v
@@ -20,6 +20,8 @@ Require Import RefinedLogMatchingLemmasInterface.
 Require Import AllEntriesLeaderLogsTermInterface.
 Require Import LeaderLogsContiguousInterface.
 Require Import OneLeaderLogPerTermInterface.
+Require Import LeaderLogsSortedInterface.
+Require Import TermSanityInterface.
 
 Section AllEntriesVotesWithLog.
 
@@ -33,7 +35,10 @@ Section AllEntriesVotesWithLog.
   Context {aellti : allEntries_leaderLogs_term_interface}.
   Context {llci : leaderLogs_contiguous_interface}.
   Context {ollpti : one_leaderLog_per_term_interface}.
-
+  Context {llsi : leaderLogs_sorted_interface}.
+  Context {tsi : term_sanity_interface}.
+  Context {rri : raft_refinement_interface}.
+  
   Definition allEntries_log (net : network) : Prop :=
     forall t e h,
       In (t, e) (allEntries (fst (nwState net h))) ->
@@ -61,6 +66,25 @@ Section AllEntriesVotesWithLog.
   Ltac destruct_update :=
     repeat (first [update_destruct_hyp|update_destruct]; subst; rewrite_update).
 
+  Definition no_entries_past_current_term_host_lifted net :=
+    forall (h : name) e,
+      In e (log (snd (nwState net h))) ->
+      eTerm e <= currentTerm (snd (nwState net h)).
+
+  Lemma no_entries_past_current_term_host_lifted_invariant :
+    forall net,
+      refined_raft_intermediate_reachable net ->
+      no_entries_past_current_term_host_lifted net.
+  Proof.
+    unfold no_entries_past_current_term_host_lifted.
+    pose proof deghost_spec.
+    do 4 intro.
+    repeat find_reverse_higher_order_rewrite.
+    eapply lift_prop; eauto.
+    intros.
+    find_apply_lem_hyp no_entries_past_current_term_invariant; eauto.
+  Qed.
+  
   Lemma appendEntries_haveNewEntries_false :
     forall net p t n pli plt es ci h e,
       refined_raft_intermediate_reachable net ->
@@ -93,6 +117,186 @@ Section AllEntriesVotesWithLog.
       t <= currentTerm (snd (nwState net h)).
   Proof.
     admit.
+  Qed.
+
+  Lemma maxIndex_le :
+    forall l1 l2,
+      sorted l1 ->
+      contiguous_range_exact_lo l1 0 ->
+      findAtIndex l1 (maxIndex l2) = None ->
+      l2 = nil
+      \/ (exists e, In e l2 /\ eIndex e = 0)
+      \/ maxIndex l1 <= maxIndex l2.
+  Proof.
+    intros. destruct l2; intuition.
+    simpl in *. right.
+    destruct l1; intuition.
+    find_copy_eapply_lem_hyp findAtIndex_None; simpl in *; eauto.
+    unfold contiguous_range_exact_lo in *.
+    simpl in *. intuition.
+    destruct (lt_eq_lt_dec 0 (eIndex e)); intuition; eauto.
+    destruct (lt_eq_lt_dec (eIndex e0) (eIndex e)); intuition.
+    exfalso. repeat break_if; do_bool; intuition.
+    match goal with
+      | H : forall _, _ < _ <= _ -> _ |- _ =>
+        specialize (H (eIndex e))
+    end; conclude_using omega.
+    simpl in *. break_exists. intuition; subst; intuition.
+    eapply findAtIndex_None; eauto.
+  Qed.
+
+  Lemma maxIndex_le' :
+    forall l1 l2 i,
+      sorted l1 ->
+      contiguous_range_exact_lo l1 0 ->
+      l2 <> nil ->
+      contiguous_range_exact_lo l2 i ->
+      findAtIndex l1 (maxIndex l2) = None ->
+      maxIndex l1 <= maxIndex l2.
+  Proof.
+    intros. find_eapply_lem_hyp maxIndex_le; intuition; eauto.
+    break_exists. intuition.
+    unfold contiguous_range_exact_lo in *.
+    intuition.
+    find_insterU. conclude_using eauto. omega.
+  Qed.
+                                 
+  Lemma sorted_app_in_in :
+    forall l1 l2 e e',
+      sorted (l1 ++ l2) ->
+      In e l1 ->
+      In e' l2 ->
+      eIndex e' < eIndex e.
+  Proof.
+    induction l1; intros; simpl in *; intuition; eauto.
+    subst. find_insterU. conclude_using ltac:(apply in_app_iff; intuition eauto).
+    intuition.
+  Qed.
+  
+  Lemma sorted_app_sorted_app_in1_in2 :
+    forall l1 l2 l3 e e',
+      sorted (l1 ++ l3) ->
+      sorted (l2 ++ l3) ->
+      In e l1 ->
+      In e' (l2 ++ l3) ->
+      eIndex e' = eIndex e ->
+      In e' l2.
+  Proof.
+    intros. do_in_app. intuition.
+    match goal with
+      | H : sorted (?l ++ ?l'), _ : In _ ?l, _ : In _ ?l' |- _ =>
+        eapply sorted_app_in_in in H
+    end; eauto.  omega.
+  Qed.
+
+  Lemma sorted_app_sorted_app_in1_in2_prefix :
+    forall l1 l2 l3 l4 e e',
+      sorted (l1 ++ l3) ->
+      sorted (l2 ++ l4) ->
+      Prefix l4 l3 ->
+      In e l1 ->
+      In e' (l2 ++ l4) ->
+      eIndex e' = eIndex e ->
+      In e' l2.
+  Proof.
+    intros. do_in_app. intuition.
+    find_eapply_lem_hyp Prefix_In; [|eauto].
+    match goal with
+      | H : sorted (?l ++ ?l'), _ : In _ ?l, _ : In _ ?l' |- _ =>
+        eapply sorted_app_in_in in H
+    end; eauto. omega.
+  Qed.
+  
+  Lemma sorted_app_in2_in2 :
+    forall l1 l2 e e',
+      sorted (l1 ++ l2) ->
+      In e' (l1 ++ l2) ->
+      In e l2 ->
+      eIndex e' = eIndex e ->
+      In e' l2.
+  Proof.
+    intros. do_in_app. intuition.
+    match goal with
+      | H : sorted (?l ++ ?l'), _ : In _ ?l, _ : In _ ?l' |- _ =>
+        eapply sorted_app_in_in in H
+    end; eauto.  omega.
+  Qed.
+
+  
+(*  Lemma sorted_app_in3_in4_prefix :
+    forall l1 l2 l3 l4 e e',
+      sorted (l1 ++ l3) ->
+      sorted (l2 ++ l4) ->
+      Prefix l4 l3 ->
+      In e l3 ->
+      In e' (l2 ++ l4) ->
+      eIndex e' = eIndex e ->
+      In e' l4.
+  Proof.
+    intros. do_in_app. intuition.
+    match goal with
+      | H : sorted (?l ++ ?l'), _ : In _ ?l, _ : In _ ?l' |- _ =>
+        eapply sorted_app_in_in in H
+    end; eauto.  omega.
+  Qed.
+  *)
+  Lemma sorted_term_index_le :
+    forall l e e',
+      sorted l ->
+      In e l ->
+      In e' l ->
+      eTerm e' < eTerm e ->
+      eIndex e' <= eIndex e.
+  Proof.
+    induction l; intros; simpl in *; intuition; subst_max; intuition.
+    - find_apply_hyp_hyp. intuition.
+    - find_apply_hyp_hyp. intuition.
+  Qed.
+  Lemma term_ne_in_l2 :
+    forall l e e' l1 l2,
+      sorted l ->
+      In e l ->
+      (forall e', In e' l -> eTerm e' <= eTerm e) ->
+      removeAfterIndex l (eIndex e) = l1 ++ l2 ->
+      (forall e', In e' l1 -> eTerm e' = eTerm e) ->
+      In e' l ->
+      eTerm e' <> eTerm e ->
+      In e' l2.
+  Proof.
+    intros.
+    assert (eIndex e' <= eIndex e) by
+        (eapply sorted_term_index_le; eauto;
+         find_apply_hyp_hyp;
+         destruct (lt_eq_lt_dec (eTerm e') (eTerm e)); intuition).
+    find_eapply_lem_hyp removeAfterIndex_le_In; eauto.
+    repeat find_rewrite.
+    do_in_app. intuition.
+    find_apply_hyp_hyp. intuition.
+  Qed.
+
+  Lemma Prefix_maxIndex_eq :
+    forall l l',
+      Prefix l l' ->
+      l <> nil ->
+      maxIndex l = maxIndex l'.
+  Proof.
+    intros.
+    induction l; simpl in *; intuition.
+    break_match; intuition. subst. simpl. auto.
+  Qed.
+
+  Lemma sorted_gt_maxIndex :
+    forall e l1 l2,
+      sorted (e :: l1 ++ l2) ->
+      l2 <> nil ->
+      maxIndex l2 < eIndex e.
+  Proof.
+    intros; induction l1; simpl in *; intuition.
+    - destruct l2; simpl in *; intuition.
+      match goal with
+        | H : forall _, ?e = _ \/ _ -> _ |- _ =>
+          specialize (H e)
+      end; intuition.
   Qed.
   
   Lemma allEntries_log_append_entries :
@@ -135,15 +339,9 @@ Section AllEntriesVotesWithLog.
         intuition;
           [break_exists; intuition;
            find_eapply_lem_hyp leaderLogs_contiguous_invariant; eauto; omega|].
-        subst.
-        match goal with
-          | H : In _ _ -> False |- _ =>
-            apply H
-        end.
-        repeat find_rewrite.
-        intuition.
+        subst. repeat find_rewrite. intuition.
       + subst.
-        find_eapply_lem_hyp allEntries_leaderLogs_term_invariant. intuition.
+        find_eapply_lem_hyp allEntries_leaderLogs_term_invariant; eauto. intuition.
         * subst. exfalso.
           find_copy_eapply_lem_hyp logs_leaderLogs_invariant; eauto.
           find_copy_eapply_lem_hyp append_entries_leaderLogs_invariant; eauto.
@@ -154,8 +352,8 @@ Section AllEntriesVotesWithLog.
           find_eapply_lem_hyp one_leaderLog_per_term_invariant; eauto;
           conclude_using eauto. subst.
           match goal with
-          | H : In _ _ -> False |- _ =>
-            apply H
+            | H : In _ _ -> False |- _ =>
+              apply H
           end.
           find_copy_eapply_lem_hyp entries_sorted_invariant; eauto.
           unfold entries_sorted in *.
@@ -167,11 +365,484 @@ Section AllEntriesVotesWithLog.
           end.
           repeat find_rewrite.
           do_in_app; intuition.
-          assert (exists e', eIndex e' = eIndex e /\ In e' (x1 ++ x4)).
-          eapply entries_contiguous_nw_invariant; eauto.
-          intuition; [eapply entries_contiguous_invariant; eauto|].
-  Admitted.
-        
+          assert (exists e', eIndex e' = eIndex e /\ In e' (x1 ++ x4)) by
+              (eapply entries_contiguous_nw_invariant; eauto;
+               intuition; [eapply entries_contiguous_invariant; eauto|];
+               eapply le_trans; [eapply maxIndex_is_max; eauto|];
+               eapply maxIndex_le'; eauto;
+               [eapply entries_contiguous_invariant; eauto|
+                eapply entries_contiguous_nw_invariant; eauto]).
+          break_exists. intuition.
+          find_copy_eapply_lem_hyp sorted_app_sorted_app_in1_in2. Focus 5. eauto. Focus 4. eauto.
+          all:(try solve [eapply entries_sorted_nw_invariant; eauto]).
+          all:(try solve [repeat find_reverse_rewrite; eauto using removeAfterIndex_sorted]).
+          find_apply_hyp_hyp.
+          find_eapply_lem_hyp entries_match_nw_host_invariant; eauto; repeat conclude_using eauto.
+          match goal with
+            | H : eIndex _ = eIndex _ |- _ =>
+              eapply uniqueIndices_elim_eq in H
+          end; eauto using sorted_uniqueIndices.
+          subst. auto.
+        * exfalso.
+          find_copy_eapply_lem_hyp append_entries_leaderLogs_invariant; eauto.
+          break_exists; intuition;
+          [break_exists; intuition;
+           find_eapply_lem_hyp leaderLogs_contiguous_invariant; eauto; omega|].
+          subst. clean.
+          find_eapply_lem_hyp one_leaderLog_per_term_invariant; eauto;
+          conclude_using eauto. subst.
+          match goal with
+            | H : In _ _ -> False |- _ =>
+              apply H
+          end.
+          repeat find_rewrite. apply in_app_iff; intuition.
+    - subst.
+      find_copy_eapply_lem_hyp allEntries_term_sanity_invariant; eauto.
+      destruct (lt_eq_lt_dec t0 t); intuition; unfold ghost_data in *; simpl in *; try omega.
+      + find_eapply_lem_hyp append_entries_leaderLogs_invariant; eauto.
+        break_exists. break_and.
+        match goal with
+          | H : In (?t, ?ll) (leaderLogs (fst (nwState _ ?leader))) |- _ =>
+            (exists t, leader, ll)
+        end. find_higher_order_rewrite.
+        split;
+          [subst; find_higher_order_rewrite;
+            destruct_update; simpl in *;
+            eauto; rewrite update_elections_data_appendEntries_leaderLogs; eauto|];
+          split; auto.
+        intuition;
+          [break_exists; intuition;
+           find_eapply_lem_hyp leaderLogs_contiguous_invariant; eauto; omega|].
+        subst. repeat find_rewrite. intuition.
+      + subst.
+        find_eapply_lem_hyp allEntries_leaderLogs_term_invariant; eauto. intuition.
+        * { subst. exfalso.
+            find_copy_eapply_lem_hyp logs_leaderLogs_invariant; eauto.
+            find_copy_eapply_lem_hyp append_entries_leaderLogs_invariant; eauto.
+            break_exists; intuition;
+            [break_exists; intuition;
+             find_eapply_lem_hyp leaderLogs_contiguous_invariant; eauto; omega|].
+            subst. clean.
+            find_eapply_lem_hyp one_leaderLog_per_term_invariant; eauto;
+            conclude_using eauto. subst.
+            match goal with
+              | H : In _ _ -> False |- _ =>
+                apply H
+            end.
+            find_copy_eapply_lem_hyp entries_sorted_invariant; eauto.
+            unfold entries_sorted in *.
+            repeat find_rewrite.
+            match goal with
+              | _ : removeAfterIndex ?l (eIndex ?e) = _ |- _ =>
+                assert (In e (removeAfterIndex l (eIndex e))) by
+                    (eapply removeAfterIndex_le_In; eauto)
+            end.
+            repeat find_rewrite.
+            do_in_app; intuition.
+            find_apply_lem_hyp findAtIndex_elim. intuition.
+            find_copy_apply_lem_hyp maxIndex_non_empty.
+            break_exists.
+            intuition.
+            match goal with
+              | _ : In ?e' (log _), _ : maxIndex ?l = eIndex ?e' |- _ =>
+                destruct (le_lt_dec (eIndex e) (maxIndex l))
+            end.
+            - assert (exists e', eIndex e' = eIndex e /\ In e' (x1 ++ x4)) by
+                  (eapply entries_contiguous_nw_invariant; eauto; intuition;
+                   eapply entries_gt_0_invariant; eauto).
+              break_exists. intuition.
+              find_copy_eapply_lem_hyp sorted_app_sorted_app_in1_in2. Focus 5. eauto. Focus 4. eauto.
+              all:(try solve [eapply entries_sorted_nw_invariant; eauto]).
+              all:(try solve [repeat find_reverse_rewrite; eauto using removeAfterIndex_sorted]).
+              find_apply_hyp_hyp.
+              find_eapply_lem_hyp entries_match_nw_host_invariant; eauto; repeat conclude_using eauto.
+              match goal with
+                | H : eIndex _ = eIndex _ |- _ =>
+                  eapply uniqueIndices_elim_eq in H
+              end; eauto using sorted_uniqueIndices.
+              subst. auto.
+            - exfalso.
+              repeat find_rewrite.
+              match goal with
+                | _ : eIndex ?e' = eIndex ?x,
+                  _ : eIndex ?x < ?i,
+                  _ : context [removeAfterIndex ?l ?i] |- _ =>
+                  assert (In e' (removeAfterIndex l i)) by
+                      (eapply removeAfterIndex_le_In; auto; omega)
+              end.
+              repeat find_rewrite.
+              do_in_app. intuition.
+              + find_copy_eapply_lem_hyp sorted_app_sorted_app_in1_in2. Focus 4. eauto.
+                all:eauto.
+                all:(try solve [eapply entries_sorted_nw_invariant; eauto]).
+                all:(try solve [repeat find_reverse_rewrite; eauto using removeAfterIndex_sorted]).
+                repeat find_apply_hyp_hyp. repeat find_rewrite. intuition.
+              + find_eapply_lem_hyp leaderLogs_sorted_invariant; eauto.
+                find_copy_eapply_lem_hyp sorted_app_in2_in2. Focus 3. eauto.
+                all:eauto.
+                all:(try solve [eapply entries_sorted_nw_invariant; eauto]).
+                match goal with
+                  | H : eIndex ?e1 = eIndex ?e2, _ : In ?e1 ?ll, _ : In ?e2 ?ll |- _ =>
+                    eapply uniqueIndices_elim_eq with (xs0 := ll) in H
+                end; eauto using sorted_uniqueIndices.
+                subst. intuition.
+          }
+        * exfalso.
+          find_copy_eapply_lem_hyp append_entries_leaderLogs_invariant; eauto.
+          break_exists; intuition;
+          [break_exists; intuition;
+           find_eapply_lem_hyp leaderLogs_contiguous_invariant; eauto; omega|].
+          subst. clean.
+          find_eapply_lem_hyp one_leaderLog_per_term_invariant; eauto;
+          conclude_using eauto. subst.
+          match goal with
+            | H : In _ _ -> False |- _ =>
+              apply H
+          end.
+          repeat find_rewrite. apply in_app_iff; intuition.
+    - find_copy_eapply_lem_hyp allEntries_term_sanity_invariant; eauto.
+      destruct (lt_eq_lt_dec t0 t); intuition; unfold ghost_data in *; simpl in *; try omega.
+      + match goal with
+          | H : context [pBody] |- _ =>
+            copy_eapply append_entries_leaderLogs_invariant H
+        end; eauto.
+        break_exists. break_and. subst.
+        match goal with
+          | H : In (?t, ?ll) (leaderLogs (fst (nwState _ ?leader))) |- _ =>
+            (exists t, leader, ll)
+        end.
+        split;
+          [find_higher_order_rewrite;
+            destruct_update; simpl in *;
+            eauto; rewrite update_elections_data_appendEntries_leaderLogs; eauto|];
+          split; auto. intuition; subst.
+        * find_false.
+          apply in_app_iff. right. eapply removeAfterIndex_le_In; eauto.
+          find_eapply_lem_hyp leaderLogs_sorted_invariant; eauto.
+          eapply le_trans; [eapply maxIndex_is_max; eauto|]. omega.
+        * {
+            break_exists. intuition. unfold Prefix_sane in *. intuition.
+            - destruct (le_lt_dec (eIndex e) (eIndex x3)).
+              + match goal with
+                  | H : In e _ -> False |- _ => apply H
+                end.
+                apply in_app_iff. right. apply removeAfterIndex_le_In; auto.
+              + match goal with
+                  | H : In e _ -> False |- _ => apply H
+                end.
+                apply in_app_iff. left.
+                apply in_app_iff. right.
+                find_eapply_lem_hyp leaderLogs_sorted_invariant; eauto.
+                eapply prefix_contiguous; eauto.
+                find_copy_eapply_lem_hyp entries_sorted_nw_invariant; eauto.
+                eapply contiguous_app; eauto.
+                eapply entries_contiguous_nw_invariant; eauto.
+            - find_false.
+              repeat find_rewrite.
+              apply in_app_iff. right.
+              find_eapply_lem_hyp leaderLogs_sorted_invariant; eauto.
+              apply removeAfterIndex_le_In; auto.
+              eapply maxIndex_is_max; eauto.
+          }
+        * find_false. intuition.
+      + subst.
+        find_eapply_lem_hyp allEntries_leaderLogs_term_invariant; eauto. intuition.
+        * { subst. exfalso.
+            find_copy_eapply_lem_hyp logs_leaderLogs_invariant; eauto.
+            find_copy_eapply_lem_hyp append_entries_leaderLogs_invariant; eauto.
+            break_exists. break_and.
+            find_eapply_lem_hyp one_leaderLog_per_term_invariant; eauto.
+            conclude_using eauto. subst. intuition.
+            - repeat find_rewrite.
+              destruct (le_lt_dec (eIndex e) (eIndex x6)).
+              + match goal with
+                  | H : In e _ -> False |- _ => apply H
+                end.
+                apply in_app_iff. right. apply removeAfterIndex_le_In; auto.
+              + match goal with
+                  | H : In e _ -> False |- _ => apply H
+                end.
+                apply in_app_iff. left.
+                find_copy_eapply_lem_hyp entries_sorted_invariant.
+                find_eapply_lem_hyp maxIndex_le'; eauto;
+                [|eapply entries_contiguous_invariant; eauto|eapply entries_contiguous_nw_invariant; eauto].
+                find_copy_eapply_lem_hyp entries_contiguous_nw_invariant; eauto.
+                unfold contiguous_range_exact_lo in *.
+                break_and.
+                find_copy_eapply_lem_hyp entries_sorted_invariant.
+                match goal with
+                  | H : forall _, _ < _ <= _ -> _ |- _ =>
+                    specialize (H (eIndex e));
+                      conclude_using ltac:(intuition; eapply le_trans; [eapply maxIndex_is_max; eauto|]; eauto)
+                end.
+                break_exists. break_and.
+                match goal with
+                  | H : eIndex ?x = eIndex e |- _ =>
+                    copy_eapply entries_match_nw_host_invariant H
+                end; eauto.
+                find_copy_eapply_lem_hyp leaderLogs_sorted_invariant; eauto.
+                conclude_using
+                  ltac:(match goal with
+                          | H : _ |- _ => apply H
+                        end; do_in_app; intuition;
+                        match goal with
+                          | H : In ?x _ |- In ?x _ =>
+                            copy_eapply Prefix_maxIndex H
+                        end; [|idtac|eauto]; eauto; omega).
+                conclude_using eauto. conclude_using auto.
+                match goal with
+                  | H : _ = _ |- _ =>
+                    eapply uniqueIndices_elim_eq in H
+                end; eauto; eauto using sorted_uniqueIndices.
+                subst. auto.
+            - break_exists. break_and.
+              destruct (le_lt_dec (eIndex e) (eIndex x6)).
+              + match goal with
+                  | H : In e _ -> False |- _ => apply H
+                end.
+                apply in_app_iff. right. apply removeAfterIndex_le_In; auto.
+              + match goal with
+                  | _ : removeAfterIndex _ (eIndex ?e) = ?l |- _ =>
+                    assert (In e l) by (repeat find_reverse_rewrite;
+                                        eapply removeAfterIndex_le_In; auto)
+                end.
+                find_copy_eapply_lem_hyp entries_sorted_invariant.
+                assert (exists e', eIndex e' = eIndex e /\ In e' (x1 ++ x2)) by
+                      (eapply entries_contiguous_nw_invariant; eauto;
+                       intuition;
+                       eapply le_trans; [eapply maxIndex_is_max; eauto|];
+                       eapply maxIndex_le'; eauto;
+                       [eapply entries_contiguous_invariant; eauto|
+                        eapply entries_contiguous_nw_invariant; eauto]).
+                do_in_app. intuition.
+                * break_exists. break_and.
+                  match goal with
+                    | H : eIndex _ = eIndex _ |- _ =>
+                      copy_eapply sorted_app_sorted_app_in1_in2_prefix H
+                  end; eauto.
+                  all:try solve [repeat find_reverse_rewrite; eauto using removeAfterIndex_sorted].
+                  all:try solve [eapply entries_sorted_nw_invariant; eauto].
+                  find_apply_hyp_hyp.
+                  match goal with
+                    | H : In e _ -> False |- _ => apply H
+                  end.
+                  apply in_app_iff. left.
+                  match goal with
+                    | H : eIndex _ = eIndex _ |- _ =>
+                      copy_eapply entries_match_nw_host_invariant H
+                  end; eauto. concludes. repeat conclude_using eauto.
+                  match goal with
+                    | H : eIndex _ = eIndex _ |- _ =>
+                      copy_eapply uniqueIndices_elim_eq H
+                  end; eauto using sorted_uniqueIndices. subst. auto.
+                * find_copy_eapply_lem_hyp leaderLogs_sorted_invariant; eauto.
+                  unfold Prefix_sane in *.
+                  intuition; [|find_eapply_lem_hyp maxIndex_is_max; eauto; omega].
+                  find_eapply_lem_hyp prefix_contiguous. Focus 2. eauto.
+                  all:eauto.
+                  all:try solve [eapply contiguous_app; [|eapply entries_contiguous_nw_invariant; eauto];
+                                 eapply entries_sorted_nw_invariant; eauto].
+                  match goal with
+                    | H : In e _ -> False |- _ => apply H
+                  end. intuition.
+            - subst.
+              destruct (le_lt_dec (eIndex e) (eIndex x6)).
+              + match goal with
+                  | H : In e _ -> False |- _ => apply H
+                end.
+                apply in_app_iff. right. apply removeAfterIndex_le_In; auto.
+              + match goal with
+                  | _ : removeAfterIndex _ (eIndex ?e) = ?l |- _ =>
+                    assert (In e l) by (repeat find_reverse_rewrite;
+                                        eapply removeAfterIndex_le_In; auto)
+                end.
+                find_copy_eapply_lem_hyp entries_sorted_invariant.
+                assert (exists e', eIndex e' = eIndex e /\ In e' (x1 ++ x4)) by
+                      (eapply entries_contiguous_nw_invariant; eauto;
+                       intuition;
+                       eapply le_trans; [eapply maxIndex_is_max; eauto|];
+                       eapply maxIndex_le'; eauto;
+                       [eapply entries_contiguous_invariant; eauto|
+                        eapply entries_contiguous_nw_invariant; eauto]).
+                do_in_app. intuition.
+                * break_exists. break_and.
+                  match goal with
+                    | H : eIndex _ = eIndex _ |- _ =>
+                      copy_eapply sorted_app_sorted_app_in1_in2 H
+                  end; eauto.
+                  all:try solve [repeat find_reverse_rewrite; eauto using removeAfterIndex_sorted].
+                  all:try solve [eapply entries_sorted_nw_invariant; eauto].
+                  find_apply_hyp_hyp.
+                  match goal with
+                    | H : In e _ -> False |- _ => apply H
+                  end.
+                  apply in_app_iff. left.
+                  match goal with
+                    | H : eIndex _ = eIndex _ |- _ =>
+                      copy_eapply entries_match_nw_host_invariant H
+                  end; eauto. concludes. repeat conclude_using eauto.
+                  match goal with
+                    | H : eIndex _ = eIndex _ |- _ =>
+                      copy_eapply uniqueIndices_elim_eq H
+                  end; eauto using sorted_uniqueIndices. subst. auto.
+                * match goal with
+                    | H : In e _ -> False |- _ => apply H
+                  end. intuition.
+          }
+        * { exfalso.
+            find_copy_eapply_lem_hyp append_entries_leaderLogs_invariant; eauto.
+            break_exists; intuition. subst.
+            copy_eapply_prop_hyp append_entries_leaderLogs pBody; eauto.
+            break_exists; break_and.
+            subst. 
+            find_eapply_lem_hyp one_leaderLog_per_term_invariant; eauto;
+            conclude_using eauto. subst.
+            match goal with
+              | H : In _ _ -> False |- _ =>
+                apply H
+            end.
+            find_copy_apply_lem_hyp leaderLogs_sorted_invariant; auto.
+            find_copy_apply_lem_hyp maxIndex_is_max; auto. 
+            destruct (le_lt_dec (eIndex e) (eIndex x1));
+              [apply in_app_iff; right; eapply removeAfterIndex_le_In; eauto|].
+            repeat find_rewrite. apply in_app_iff; intuition.
+            - omega.
+            - break_exists; break_and.
+              unfold Prefix_sane in *. break_or_hyp; try omega.
+              left; apply in_app_iff; right.
+              eapply prefix_contiguous; eauto.
+              eapply contiguous_app; [|eapply entries_contiguous_nw_invariant; eauto];
+              eapply entries_sorted_nw_invariant; eauto.
+            - subst. intuition.
+          }
+    - find_copy_eapply_lem_hyp allEntries_term_sanity_invariant; eauto.
+      destruct (lt_eq_lt_dec t0 t); intuition; unfold ghost_data in *; simpl in *; try omega.
+      + match goal with
+          | H : context [pBody] |- _ =>
+            copy_eapply append_entries_leaderLogs_invariant H
+        end; eauto.
+        break_exists. break_and. subst.
+        match goal with
+          | H : In (?t, ?ll) (leaderLogs (fst (nwState _ ?leader))) |- _ =>
+            (exists t, leader, ll)
+        end.
+        split;
+          [find_higher_order_rewrite;
+            destruct_update; simpl in *;
+            eauto; rewrite update_elections_data_appendEntries_leaderLogs; eauto|];
+          split; auto. intuition; subst.
+        * find_false.
+          apply in_app_iff. right. eapply removeAfterIndex_le_In; eauto.
+          find_eapply_lem_hyp leaderLogs_sorted_invariant; eauto.
+          eapply le_trans; [eapply maxIndex_is_max; eauto|]. omega.
+        * {
+            break_exists. intuition. unfold Prefix_sane in *. intuition.
+            - destruct (le_lt_dec (eIndex e) (eIndex x4)).
+              + match goal with
+                  | H : In e _ -> False |- _ => apply H
+                end.
+                apply in_app_iff. right. apply removeAfterIndex_le_In; auto.
+              + match goal with
+                  | H : In e _ -> False |- _ => apply H
+                end.
+                apply in_app_iff. left.
+                apply in_app_iff. right.
+                find_eapply_lem_hyp leaderLogs_sorted_invariant; eauto.
+                eapply prefix_contiguous; eauto.
+                find_copy_eapply_lem_hyp entries_sorted_nw_invariant; eauto.
+                eapply contiguous_app; eauto.
+                eapply entries_contiguous_nw_invariant; eauto.
+            - find_false.
+              repeat find_rewrite.
+              apply in_app_iff. right.
+              find_eapply_lem_hyp leaderLogs_sorted_invariant; eauto.
+              apply removeAfterIndex_le_In; auto.
+              eapply maxIndex_is_max; eauto.
+          }
+        * find_false. intuition.
+      + subst.
+        find_eapply_lem_hyp allEntries_leaderLogs_term_invariant; eauto. intuition.
+        * { subst. exfalso.
+            find_copy_eapply_lem_hyp logs_leaderLogs_invariant; eauto.
+            find_copy_eapply_lem_hyp append_entries_leaderLogs_invariant; eauto.
+            break_exists. break_and.
+            find_eapply_lem_hyp one_leaderLog_per_term_invariant; eauto.
+            conclude_using eauto. subst.
+            find_eapply_lem_hyp le_antisym; eauto.
+            destruct x1.
+            - simpl in *. destruct x2; simpl in *; auto.
+              break_match; auto.
+              match goal with
+                | H : _ \/ (exists _, _) \/ _ |- _ =>
+                  clear H
+              end.
+              break_and. subst.
+              cut (e1 = x6); intros; subst; auto.
+              find_apply_lem_hyp findAtIndex_elim.
+              break_and.
+              find_copy_apply_lem_hyp entries_sorted_invariant.
+              eapply uniqueIndices_elim_eq; eauto using sorted_uniqueIndices.
+              eapply removeAfterIndex_in with (i := (eIndex e)).
+              unfold raft_data, ghost_data in *; simpl in *.
+              unfold raft_data, ghost_data in *; simpl in *.
+              repeat find_rewrite. intuition.
+            - simpl in *.
+              match goal with
+                | H : forall _, ?e = _ \/ _ -> _ |- _ =>
+                  specialize (H e)
+              end. conclude_using auto.
+              repeat find_rewrite.
+              find_apply_lem_hyp findAtIndex_elim. break_and.
+              find_eapply_lem_hyp term_ne_in_l2; eauto.
+              all:try solve [eapply entries_sorted_invariant; eauto].
+              all:try solve [intros; find_eapply_lem_hyp no_entries_past_current_term_host_lifted_invariant; unfold ghost_data, raft_data in *; simpl in *;
+                             unfold ghost_data, raft_data in *; simpl in *;
+                             repeat find_rewrite; eauto].
+              assert (eIndex e0 <= maxIndex x4) by
+                  (repeat find_rewrite;
+                   eapply maxIndex_is_max; eauto;
+                   eapply leaderLogs_sorted_invariant; eauto).
+              assert (eIndex x7 < eIndex e0) by
+                  (eapply entries_contiguous_nw_invariant; eauto; intuition).
+              intuition.
+              + break_exists. break_and.
+                unfold Prefix_sane in *. intuition.
+                find_copy_eapply_lem_hyp Prefix_maxIndex_eq; eauto.
+                find_eapply_lem_hyp entries_sorted_nw_invariant; eauto.
+                find_eapply_lem_hyp sorted_gt_maxIndex; eauto; omega.
+              + subst.
+                find_eapply_lem_hyp entries_sorted_nw_invariant; eauto.
+                find_eapply_lem_hyp sorted_gt_maxIndex; eauto; try omega.
+                destruct x4; simpl in *; congruence.
+          }
+        * { exfalso.
+            find_copy_eapply_lem_hyp append_entries_leaderLogs_invariant; eauto.
+            break_exists; intuition. subst.
+            copy_eapply_prop_hyp append_entries_leaderLogs pBody; eauto.
+            break_exists; break_and.
+            subst. 
+            find_eapply_lem_hyp one_leaderLog_per_term_invariant; eauto;
+            conclude_using eauto. subst.
+            match goal with
+              | H : In _ _ -> False |- _ =>
+                apply H
+            end.
+            find_copy_apply_lem_hyp leaderLogs_sorted_invariant; auto.
+            find_copy_apply_lem_hyp maxIndex_is_max; auto. 
+            destruct (le_lt_dec (eIndex e) (eIndex x2));
+              [apply in_app_iff; right; eapply removeAfterIndex_le_In; eauto|].
+            repeat find_rewrite. apply in_app_iff; intuition.
+            - omega.
+            - break_exists; break_and.
+              unfold Prefix_sane in *. break_or_hyp; try omega.
+              left; apply in_app_iff; right.
+              eapply prefix_contiguous; eauto.
+              eapply contiguous_app; [|eapply entries_contiguous_nw_invariant; eauto];
+              eapply entries_sorted_nw_invariant; eauto.
+            - subst. intuition.
+          }
+  Qed.
+  
   Instance aevwli : allEntries_votesWithLog_interface.
   Admitted.
 End AllEntriesVotesWithLog.
